Checkpoint. Simplifying LLVMEvents and DynamicValues memory parameters.

src/llvm-mem/GepM.v
@@ -1,5 +1,8 @@
 From Stdlib Require Import ZArith String List Lia.
 
+From Coq Require Import
+  Structures.Equalities.
+
 From ExtLib Require Import
      Structures.Monad
      Structures.Functor.
@@ -12,7 +15,8 @@ From Vellvm Require Import
   Utils.Tactics.
 
 From Mem Require Import
-  Addresses.MemoryAddress.
+  Addresses.MemoryAddress
+  Addresses.Provenance.
 
 From LLVM_Memory Require Import
   Sizeof
@@ -21,10 +25,10 @@ From LLVM_Memory Require Import
 Import ListNotations.
 Import MonadNotation.
 
-Module Type GEPM (Addr:ADDRESS) (ITOP : ITOP Addr) (SIZEOF:Sizeof).
+Module Type GEPM (Addr : BASIC_ADDRESS) (IP : INTPTR) (SIZEOF : Sizeof) (LLVM_Events : LLVM_INTERACTIONS Addr IP SIZEOF).
   Import Addr.
-  Import ITOP.
   Import SIZEOF.
+  Import LLVM_Events.
 
   (** ** Get Element Pointer
       Retrieve the address of a subelement of an indexable (i.e. aggregate) [dtyp] [t] (i.e. vector, array, struct, packed struct).
@@ -35,7 +39,7 @@ Module Type GEPM (Addr:ADDRESS) (ITOP : ITOP Addr) (SIZEOF:Sizeof).
       The offset is therefore incremented by this index times the size of the type of elements stored. Finally, a recursive call
       at this new offset allows for deeper unbundling of a nested structure.
    *)
-  Fixpoint handle_gep_h (t:dtyp) (off:Z) (vs:list dvalue): err Z :=
+  Fixpoint calculate_gep_offset (t:dtyp) (off:Z) (vs:list dvalue): err Z :=
     match vs with
     | v :: vs' =>
       match v with
@@ -45,7 +49,7 @@ Module Type GEPM (Addr:ADDRESS) (ITOP : ITOP Addr) (SIZEOF:Sizeof).
         match t with
         | DTYPE_Array _ ta
         | DTYPE_Vector _ ta =>
-            handle_gep_h ta (off + k * (Z.of_N (sizeof_dtyp ta))) vs'
+            calculate_gep_offset ta (off + k * (Z.of_N (sizeof_dtyp ta))) vs'
         | _ => failwith ("non-i8-indexable type")
         end
       | @DVALUE_I 32 i =>
@@ -55,14 +59,14 @@ Module Type GEPM (Addr:ADDRESS) (ITOP : ITOP Addr) (SIZEOF:Sizeof).
         match t with
         | DTYPE_Array _ ta
         | DTYPE_Vector _ ta =>
-            handle_gep_h ta (off + ks * (Z.of_N (sizeof_dtyp ta))) vs'
+            calculate_gep_offset ta (off + ks * (Z.of_N (sizeof_dtyp ta))) vs'
         | DTYPE_Struct ts =>
             let offset := fold_left (fun acc t => pad_to_align (dtyp_alignment t) acc + sizeof_dtyp t)%N
                             (firstn n ts) 0%N in
             match nth_error ts n with
             | None => failwith "overflow"
             | Some t' =>
-                handle_gep_h t' (off + Z.of_N offset) vs'
+                calculate_gep_offset t' (off + Z.of_N offset) vs'
             end
         | DTYPE_Packed_struct ts =>
           let offset := fold_left (fun acc t => acc + sizeof_dtyp t)%N
@@ -70,7 +74,7 @@ Module Type GEPM (Addr:ADDRESS) (ITOP : ITOP Addr) (SIZEOF:Sizeof).
           match nth_error ts n with
           | None => failwith "overflow"
           | Some t' =>
-            handle_gep_h t' (off + Z.of_N offset) vs'
+            calculate_gep_offset t' (off + Z.of_N offset) vs'
           end
         | _ => failwith ("non-i32-indexable type")
         end
@@ -80,7 +84,7 @@ Module Type GEPM (Addr:ADDRESS) (ITOP : ITOP Addr) (SIZEOF:Sizeof).
         match t with
         | DTYPE_Array _ ta
         | DTYPE_Vector _ ta =>
-            handle_gep_h ta (off + k * (Z.of_N (sizeof_dtyp ta))) vs'
+            calculate_gep_offset ta (off + k * (Z.of_N (sizeof_dtyp ta))) vs'
         | _ => failwith ("non-i64-indexable type")
         end
       | DVALUE_IPTR i =>
@@ -89,34 +93,108 @@ Module Type GEPM (Addr:ADDRESS) (ITOP : ITOP Addr) (SIZEOF:Sizeof).
         match t with
         | DTYPE_Array _ ta
         | DTYPE_Vector _ ta =>
-            handle_gep_h ta (off + k * (Z.of_N (sizeof_dtyp ta))) vs'
+            calculate_gep_offset ta (off + k * (Z.of_N (sizeof_dtyp ta))) vs'
         | _ => failwith ("non-iptr-indexable type")
         end
-      | _ => failwith "handle_gep_h: unsupported index type"
+      | _ => failwith "calculate_gep_offset: unsupported index type"
       end
     | [] => ret off
     end.
+
+  (* Calculate GEP offsets directly with pointer type. May not need this *)
+  Fixpoint handle_gep_ptr_h (t:dtyp) (ptr:addr) (vs:list dvalue): err addr :=
+    match vs with
+    | v :: vs' =>
+      match v with
+      | @DVALUE_I 8 i =>
+        let k := signed i in
+        let n := BinIntDef.Z.to_nat k in
+        match t with
+        | DTYPE_Array _ ta
+        | DTYPE_Vector _ ta =>
+            ptr' <- ptr_add ptr (k * (Z.of_N (sizeof_dtyp ta)));;
+            handle_gep_ptr_h ta ptr' vs'
+        | _ => failwith ("non-i8-indexable type")
+        end
+      | @DVALUE_I 32 i =>
+        let k := unsigned i in
+        let ks := signed i in
+        let n := BinIntDef.Z.to_nat k in
+        match t with
+        | DTYPE_Array _ ta
+        | DTYPE_Vector _ ta =>
+            ptr' <- ptr_add ptr (ks * (Z.of_N (sizeof_dtyp ta)));;
+            handle_gep_ptr_h ta ptr' vs'
+        | DTYPE_Struct ts =>
+            let offset := fold_left (fun acc t => pad_to_align (dtyp_alignment t) acc + sizeof_dtyp t)%N
+                            (firstn n ts) 0%N in
+            match nth_error ts n with
+            | None => failwith "overflow"
+            | Some t' =>
+                ptr' <- ptr_add ptr (Z.of_N offset);;
+                handle_gep_ptr_h t' ptr' vs'
+            end
+        | DTYPE_Packed_struct ts =>
+          let offset := fold_left (fun acc t => acc + sizeof_dtyp t)%N
+                                  (firstn n ts) 0%N in
+          match nth_error ts n with
+          | None => failwith "overflow"
+          | Some t' =>
+              ptr' <- ptr_add ptr (Z.of_N offset);;
+              handle_gep_ptr_h t' ptr' vs'
+          end
+        | _ => failwith ("non-i32-indexable type")
+        end
+      | @DVALUE_I 64 i =>
+        let k := signed i in
+        let n := BinIntDef.Z.to_nat k in
+        match t with
+        | DTYPE_Array _ ta
+        | DTYPE_Vector _ ta =>
+            ptr' <- ptr_add ptr (k * (Z.of_N (sizeof_dtyp ta)));;
+            handle_gep_ptr_h ta ptr' vs'
+        | _ => failwith ("non-i64-indexable type")
+        end
+      | DVALUE_IPTR i =>
+        let k := IP.to_Z i in
+        let n := BinIntDef.Z.to_nat k in
+        match t with
+        | DTYPE_Array _ ta
+        | DTYPE_Vector _ ta =>
+            ptr' <- ptr_add ptr (k * (Z.of_N (sizeof_dtyp ta)));;
+            handle_gep_ptr_h ta ptr' vs'
+        | _ => failwith ("non-iptr-indexable type")
+        end
+      | _ => failwith "handle_gep_ptr_h: unsupported index type"
+      end
+    | [] => ret ptr
+    end.
+
+  (* TODO: Should probably move / abstract this *)
+  Definition ptr_add_oom (a : addr) (off : Z) : OOM addr :=
+    match ptr_add a off with
+    | inl msg => Oom msg
+    | inr ptr => NoOom ptr
+    end.                  
 
   (* At the toplevel, GEP takes a [dvalue] as an argument that must contain a pointer, but no other pointer can be recursively followed.
      The pointer set the block into which we look, and the initial offset. The first index value add to the initial offset passed to [handle_gep_h] for the actual access to structured data.
    *)
   (* TODO: This should take into account padding too... May break get_consecutive_ptrs and friends. *)
   Definition handle_gep_addr (t:dtyp) (a:addr) (vs:list dvalue) : err (OOM addr) :=
-    let ptr := ptr_to_int a in
-    let prov := address_provenance a in
     match vs with
     | @DVALUE_I 8 i :: vs' =>
-      ptr' <- handle_gep_h t (ptr + Z.of_N (sizeof_dtyp t) * (signed i)) vs' ;;
-      ret (int_to_ptr ptr' prov)
+        off <- calculate_gep_offset t (Z.of_N (sizeof_dtyp t) * (signed i)) vs';;
+        ret (ptr_add_oom a off)
     | @DVALUE_I 32 i :: vs' =>
-      ptr' <- handle_gep_h t (ptr + Z.of_N (sizeof_dtyp t) * (signed i)) vs' ;;
-      ret (int_to_ptr ptr' prov)
+        off <- calculate_gep_offset t (Z.of_N (sizeof_dtyp t) * (signed i)) vs';;
+        ret (ptr_add_oom a off)
     | @DVALUE_I 64 i :: vs' =>
-      ptr' <- handle_gep_h t (ptr + Z.of_N (sizeof_dtyp t) * (signed i)) vs' ;;
-      ret (int_to_ptr ptr' prov)
+        off <- calculate_gep_offset t (Z.of_N (sizeof_dtyp t) * (signed i)) vs';;
+        ret (ptr_add_oom a off)
     | DVALUE_IPTR i :: vs' =>
-      ptr' <- handle_gep_h t (ptr + Z.of_N (sizeof_dtyp t) * (IP.to_Z i)) vs' ;;
-      ret (int_to_ptr ptr' prov)
+        off <- calculate_gep_offset t (Z.of_N (sizeof_dtyp t) * (IP.to_Z i)) vs';;
+        ret (ptr_add_oom a off)
     | [] => failwith "handle_gep_addr: no indices"
     | _ => failwith "handle_gep_addr: unsupported index type"
     end.
@@ -128,8 +206,9 @@ Module Type GEPM (Addr:ADDRESS) (ITOP : ITOP Addr) (SIZEOF:Sizeof).
     intros dt p.
     cbn.
     rewrite IP.to_Z_0.
-    replace (ptr_to_int p + Z.of_N (sizeof_dtyp dt) * 0)%Z with (ptr_to_int p) by lia.
-    rewrite int_to_ptr_ptr_to_int; auto.
+    unfold ptr_add_oom.
+    replace (Z.of_N (sizeof_dtyp dt) * 0)%Z with 0%Z by lia.
+    rewrite ptr_add_0; auto.
   Qed.
 
   Lemma handle_gep_addr_nil :
@@ -140,52 +219,88 @@ Module Type GEPM (Addr:ADDRESS) (ITOP : ITOP Addr) (SIZEOF:Sizeof).
     cbn; auto.
   Qed.
 
+  Lemma handle_gep_addr_ptr_add_ix :
+    forall (dt : dtyp) (p p' : addr) ix,
+      handle_gep_addr dt p [DVALUE_IPTR ix] = inr (ret p') ->
+      ptr_add p (Z.of_N (sizeof_dtyp dt) * IP.to_Z ix) = inr p'.
+  Proof.
+    intros dt p p' ix GEP.
+    cbn in *.
+    inv GEP.
+    unfold ptr_add_oom in H0.
+    break_match_hyp_inv; auto.
+  Qed.
+
   Lemma handle_gep_addr_ix :
     forall (dt : dtyp) (p p' : addr) ix,
       handle_gep_addr dt p [DVALUE_IPTR ix] = inr (ret p') ->
       ptr_to_int p' = (ptr_to_int p + Z.of_N (sizeof_dtyp dt) * IP.to_Z ix)%Z.
   Proof.
     intros dt p p' ix GEP.
-    cbn in *.
-    inv GEP.
-    erewrite ptr_to_int_int_to_ptr; eauto.
+    apply handle_gep_addr_ptr_add_ix in GEP.
+    erewrite <- ptr_to_int_ptr_add; eauto.
   Qed.
 
-  Lemma handle_gep_addr_ix_OOM :
+  Lemma handle_gep_addr_ptr_add_ix_OOM :
     forall (dt : dtyp) (p p' : addr) ix msg,
       handle_gep_addr dt p [DVALUE_IPTR ix] = inr (Oom msg) ->
-      exists msg',
-        int_to_ptr (ptr_to_int p + Z.of_N (sizeof_dtyp dt) * IP.to_Z ix)%Z (address_provenance p) = Oom msg'.
+      ptr_add p (Z.of_N (sizeof_dtyp dt) * IP.to_Z ix) = inl msg.
   Proof.
     intros dt p p' ix msg GEP.
     cbn in *.
-    exists msg.
-    inv GEP.
-    auto.
+    unfold ptr_add_oom in GEP.
+    break_match_hyp_inv; auto.
   Qed.
 
-  Lemma handle_gep_addr_ix' :
+  Lemma handle_gep_addr_ptr_add_ix' :
     forall (dt : dtyp) (p p' : addr) ix,
-      ret p' = int_to_ptr (ptr_to_int p + Z.of_N (sizeof_dtyp dt) * IP.to_Z ix)%Z (address_provenance p) ->
+      ptr_add p (Z.of_N (sizeof_dtyp dt) * IP.to_Z ix) = ret p' ->
       handle_gep_addr dt p [DVALUE_IPTR ix] = inr (ret p').
   Proof.
     intros dt p p' ix IX.
     cbn in *.
-    inv IX.
+    unfold ptr_add_oom.
+    rewrite IX.
     reflexivity.
   Qed.
 
-  Lemma handle_gep_addr_ix'_OOM :
+  Lemma handle_gep_addr_ptr_add_ix'_OOM :
     forall (dt : dtyp) (p p' : addr) ix msg,
-      int_to_ptr (ptr_to_int p + Z.of_N (sizeof_dtyp dt) * IP.to_Z ix)%Z (address_provenance p) = Oom msg ->
-      exists msg', handle_gep_addr dt p [DVALUE_IPTR ix] = inr (Oom msg').
+      ptr_add p (Z.of_N (sizeof_dtyp dt) * IP.to_Z ix) = inl msg ->
+      handle_gep_addr dt p [DVALUE_IPTR ix] = inr (Oom msg).
   Proof.
     intros dt p p' ix msg IX.
     cbn in *.
-    exists msg.
-    inv IX.
-    auto.
+    unfold ptr_add_oom.
+    rewrite IX.
+    reflexivity.
   Qed.
+
+  (* Lemma handle_gep_addr_ix' : *)
+  (*   forall (dt : dtyp) (p p' : addr) ix, *)
+  (*     ret p' = int_to_ptr (ptr_to_int p + Z.of_N (sizeof_dtyp dt) * IP.to_Z ix)%Z (extract_metadata p) -> *)
+  (*     handle_gep_addr dt p [DVALUE_IPTR ix] = inr (ret p'). *)
+  (* Proof. *)
+  (*   intros dt p p' ix IX. *)
+  (*   apply handle_gep_addr_ptr_add_ix'. *)
+  (*   erewrite ptr_to_int_ptr_add in IX; eauto. *)
+    
+  (*   cbn in *. *)
+  (*   inv IX. *)
+  (*   reflexivity. *)
+  (* Qed. *)
+
+  (* Lemma handle_gep_addr_ix'_OOM : *)
+  (*   forall (dt : dtyp) (p p' : addr) ix msg, *)
+  (*     int_to_ptr (ptr_to_int p + Z.of_N (sizeof_dtyp dt) * IP.to_Z ix)%Z (address_provenance p) = Oom msg -> *)
+  (*     exists msg', handle_gep_addr dt p [DVALUE_IPTR ix] = inr (Oom msg'). *)
+  (* Proof. *)
+  (*   intros dt p p' ix msg IX. *)
+  (*   cbn in *. *)
+  (*   exists msg. *)
+  (*   inv IX. *)
+  (*   auto. *)
+  (* Qed. *)
 
   (* Lemma handle_gep_addr_cons_inv : *)
   (*   forall t base_addr idx idxs final_addr, *)
@@ -287,23 +402,6 @@ Module Type GEPM (Addr:ADDRESS) (ITOP : ITOP Addr) (SIZEOF:Sizeof).
   (*   reflexivity. *)
   (* Qed. *)
 
-  Lemma handle_gep_addr_preserves_provenance :
-    forall (dt : dtyp) ixs (p p' : addr),
-      handle_gep_addr dt p ixs = inr (ret p') ->
-      address_provenance p = address_provenance p'.
-  Proof.
-    intros dt ixs.
-    induction ixs;
-      intros p p' GEP;
-      [inversion GEP|].
-
-    cbn in GEP.
-    repeat break_match_hyp_inv;
-      cbn in *;
-      symmetry;
-      eapply int_to_ptr_provenance; eauto.
-  Qed.
-
   Definition handle_gep (t:dtyp) (dv:dvalue) (vs:list dvalue) : err (OOM dvalue) :=
     match dv with
     | DVALUE_Addr a => fmap (F:=err) (fmap DVALUE_Addr) (handle_gep_addr t a vs)
@@ -311,14 +409,45 @@ Module Type GEPM (Addr:ADDRESS) (ITOP : ITOP Addr) (SIZEOF:Sizeof).
     end.
 End GEPM.
 
-Module Make (ADDR : ADDRESS) (IP : INTPTR) (SIZE : Sizeof) (Events : LLVM_INTERACTIONS(ADDR)(IP)(SIZE)) (PTOI : PTOI ADDR) (PROV : PROVENANCE ADDR) (ITOP : ITOP ADDR PROV PTOI) <: GEPM(ADDR)(PTOI)(PROV)(ITOP)(IP)(SIZE)(Events).
-  Import ADDR.
-  Import Events.
-  Import DV.
-  Import SIZE.
-  Import PTOI.
-  Import ITOP.
-  Import PROV.
+(* Module Type GEPM_EXTRA (MD : Typ) (PS : PROV_SET) (Addr : ADDRESS MD PS) (IP : INTPTR) (SIZEOF : Sizeof) (LLVM_Events : LLVM_INTERACTIONS Addr IP SIZEOF) <: GEPM. *)
+(*   Include (GEPM Addr IP SIZEOF LLVM_Events). *)
+(*   Import Addr. *)
 
-  Include GEPM (ADDR)(PTOI)(PROV)(ITOP)(IP)(SIZE)(Events).
+(*   Lemma handle_gep_addr_preserves_metadata : *)
+(*     forall (dt : dtyp) ixs (p p' : addr), *)
+(*       handle_gep_addr dt p ixs = inr (ret p') -> *)
+(*       extract_metadata p = extract_metadata p'. *)
+(*   Proof. *)
+(*     intros dt ixs. *)
+(*     induction ixs; *)
+(*       intros p p' GEP; *)
+(*       [inversion GEP|]. *)
+
+(*     cbn in GEP. *)
+(*     repeat break_match_hyp_inv; *)
+(*       cbn in *; *)
+(*       symmetry. *)
+(*       eapply int_to_ptr_provenance; eauto. *)
+(*   Qed. *)
+
+(*   Lemma handle_gep_addr_preserves_provenance : *)
+(*     forall (dt : dtyp) ixs (p p' : addr), *)
+(*       handle_gep_addr dt p ixs = inr (ret p') -> *)
+(*       address_provenance p = address_provenance p'. *)
+(*   Proof. *)
+(*     intros dt ixs. *)
+(*     induction ixs; *)
+(*       intros p p' GEP; *)
+(*       [inversion GEP|]. *)
+
+(*     cbn in GEP. *)
+(*     repeat break_match_hyp_inv; *)
+(*       cbn in *; *)
+(*       symmetry; *)
+(*       eapply int_to_ptr_provenance; eauto. *)
+(*   Qed. *)
+(* End GEPM_EXTRA. *)
+
+Module Make (ADDR : BASIC_ADDRESS) (IP : INTPTR) (SIZE : Sizeof) (Events : LLVM_INTERACTIONS(ADDR)(IP)(SIZE)) <: GEPM ADDR IP SIZE Events.
+  Include (GEPM ADDR IP SIZE Events).
 End Make.
