src/rocq/Semantics/LLVMEvents.v
@@ -162,12 +162,12 @@ Set Contextual Implicit.
 
 
 (* TODO: decouple these definitions from the instance of DVALUE and DTYP by using polymorphism not functors. *)
-Module Type LLVM_INTERACTIONS (ADDRESS_METADATA : Typ) (PS : PROV_SET) (ADDR : ADDRESS ADDRESS_METADATA PS) (IP:INTPTR) (SIZEOF : Sizeof).
+Module Type LLVM_INTERACTIONS (ADDR : NULLABLE_ADDRESS) (IP:INTPTR) (SIZEOF : Sizeof).
 
   #[global] Instance eq_dec_addr : RelDec (@eq ADDR.addr) := RelDec_from_dec _ ADDR.eq_dec.
   #[global] Instance Eqv_addr : Eqv ADDR.addr := (@eq ADDR.addr).
 
-  Module DV := DynamicValues.DVALUE(ADDRESS_METADATA)(PS)(ADDR)(IP)(SIZEOF).
+  Module DV := DynamicValues.DVALUE ADDR IP SIZEOF.
   Export DV.
 
   Section Events.
@@ -328,6 +328,6 @@ Module Type LLVM_INTERACTIONS (ADDRESS_METADATA : Typ) (PS : PROV_SET) (ADDR : A
 
 End LLVM_INTERACTIONS.
 
-Module Make(ADDRESS_METADATA : Typ) (PS : PROV_SET) (ADDR : ADDRESS ADDRESS_METADATA PS) (IP:INTPTR) (SIZEOF : Sizeof) <: LLVM_INTERACTIONS(ADDRESS_METADATA)(PS)(ADDR)(IP)(SIZEOF).
-Include LLVM_INTERACTIONS(ADDRESS_METADATA)(PS)(ADDR)(IP)(SIZEOF).
+Module Make (ADDR : NULLABLE_ADDRESS) (IP:INTPTR) (SIZEOF : Sizeof) <: LLVM_INTERACTIONS ADDR IP SIZEOF.
+  Include (LLVM_INTERACTIONS ADDR IP SIZEOF).
 End Make.
